several inductive sort definition with Niels (#33)

sort.v
@@ -5,9 +5,7 @@ Require Import List.
 
 Require Import comparable.
 
-(* TODO: Help Wanted
-Use /\ and \/ to define a more compact version of the is_sorted property
-*)
+
 (* is_sorted is a property that says whether a list is sorted *)
 Fixpoint is_sorted {X: Set} {tc: comparable X} (xs: list X) : Prop :=
   match xs with
@@ -15,14 +13,119 @@ Fixpoint is_sorted {X: Set} {tc: comparable X} (xs: list X) : Prop :=
   | (x'::xs') => match xs' with
     | nil => True
     | (x''::xs'') => match compare x' x'' with
+      | Eq => True
+      | Lt => True
       | Gt => False
-      | _ => is_sorted xs'
       end
     end
   end.
 
-Theorem sort_incremental: forall {X: Set} {tc: comparable X} (xs: list X)  (x: X) {s : is_sorted (x :: xs)},
-  is_sorted xs.
+Inductive is_sorted' {X: Set} {tc: comparable X} : list X -> Prop :=
+  | empty_sorted' : is_sorted' nil
+  | singleton_sorted' (x: X) : is_sorted' (x :: nil)
+  | lessthan_sorted'
+    (x: X)
+    (y: X)
+    (c : compare x y = Lt)
+    (xs: list X)
+    (s: is_sorted' (y :: xs))
+    : is_sorted' (x :: y :: xs)
+  | equal_sorted'
+    (x: X)
+    (y: X)
+    (c : compare x y = Eq)
+    (xs: list X)
+    (s: is_sorted' (y :: xs))
+    : is_sorted' (x :: y :: xs)
+.
+
+Inductive is_sorted'' {X: Set} {tc: comparable X} : list X -> Prop :=
+  | empty_sorted'' : is_sorted'' nil
+  | singleton_sorted'' : forall x, is_sorted'' (x :: nil)
+  | lessthan_sorted''
+    : forall (x: X) (xs: list X),
+      (exists (y: X) (ys: list X),
+      xs = (y :: ys)
+      /\ compare x y = Lt)
+      /\ is_sorted'' xs
+      -> is_sorted'' (x :: xs)
+  | equal_sorted''
+    : forall (x: X) (xs: list X),
+      (exists (y: X) (ys: list X),
+      xs = (y :: ys)
+      /\ compare x y = Eq)
+      /\ is_sorted'' xs
+      -> is_sorted'' (x :: xs)
+.
+
+Lemma tail_of_is_sorted_is_sorted:
+  forall {X: Set}
+  {tc: comparable X}
+  (x: X)
+  (xs: list X),
+  is_sorted (x :: xs) -> is_sorted xs.
+Proof.
+(* TODO: Good First Issue *)
+Admitted.
+
+Lemma tail_of_is_sorted'_is_sorted':
+  forall {X: Set}
+  {tc: comparable X}
+  (x: X)
+  (xs: list X),
+  is_sorted' (x :: xs) -> is_sorted' xs.
+Proof.
+(* TODO: Good First Issue *)
+Admitted.
+
+Lemma tail_of_is_sorted''_is_sorted'':
+  forall {X: Set}
+  {tc: comparable X}
+  (x: X)
+  (xs: list X),
+  is_sorted'' (x :: xs) -> is_sorted'' xs.
+Proof.
+(* TODO: Good First Issue *)
+Admitted.
+
+Theorem is_sorted_and_is_sorted'_are_equivalent : forall {X: Set} {tc: comparable X} (xs: list X),
+  is_sorted xs <-> is_sorted' xs.
+Proof.
+intros.
+split.
+- induction xs as [(*nil*)| x0 xs' IH].
+  + simpl.
+    intros.
+    exact empty_sorted'.
+  + induction xs' as [(*nil*)| x1 xs''].
+    * simpl.
+      intros.
+      exact (singleton_sorted' x0).
+    * intros.
+      assert (is_sorted (x1 :: xs'')).
+      -- apply tail_of_is_sorted_is_sorted with (x := x0) (xs := (x1 :: xs'')).
+         assumption.
+      -- apply IH in H0.
+         simpl in H.
+         destruct (compare x0 x1) eqn:c.
+         ++ refine (equal_sorted' _ _ _).
+            ** exact c.
+            ** exact H0.
+         ++ exact (lessthan_sorted' _ c H0).
+         ++ contradiction.
+- induction xs as [(*nil*)| x0 xs' IH].
+  + simpl.
+    intros.
+    trivial.
+  + intros.
+    inversion H.
+    * simpl. trivial.
+    * simpl. rewrite c. trivial.
+    * simpl. rewrite c. trivial.
+Qed.
+
+Theorem is_sorted'_and_is_sorted''_are_equivalent : forall {X: Set} {tc: comparable X} (xs: list X),
+  is_sorted' xs <-> is_sorted'' xs.
 Proof.
 (* TODO: Good First Issue *)
 Admitted.
